Added sender wrapper. Renamed sender fixrec function and revised sender and testing theory. Completed proofs for additional properties have to be merged again.

CaseStudies/ABP/Sender.thy
@@ -19,613 +19,141 @@ section {* definition *}
 
 text {* input: msg from the user, acks from the receiver, ack buffer for the expected ack 
         output: msg and expected ack for the receiver *}
-fixrec tsSnd :: "'a tstream \<rightarrow> bool tstream \<rightarrow> bool discr \<rightarrow> ('a \<times> bool) tstream" where
+fixrec tsSnd_h :: "'a tstream \<rightarrow> bool tstream \<rightarrow> bool discr \<rightarrow> ('a \<times> bool) tstream" where
   (* bottom case *)
-"tsSnd\<cdot>\<bottom>\<cdot>acks\<cdot>ack = \<bottom>" |
-"tsSnd\<cdot>msg\<cdot>\<bottom>\<cdot>ack = \<bottom>" |
+"tsSnd_h\<cdot>\<bottom>\<cdot>acks\<cdot>ack = \<bottom>" |
+"tsSnd_h\<cdot>msg\<cdot>\<bottom>\<cdot>ack = \<bottom>" |
 
   (* if an input and ack from the receiver *)
-"msg\<noteq>\<bottom> \<Longrightarrow> acks\<noteq>\<bottom> \<Longrightarrow> tsSnd\<cdot>(tsLscons\<cdot>(up\<cdot>(uMsg\<cdot>m))\<cdot>msg)\<cdot>(tsLscons\<cdot>(up\<cdot>(uMsg\<cdot>a))\<cdot>acks)\<cdot>ack = 
+"msg \<noteq> \<bottom> \<Longrightarrow> acks \<noteq> \<bottom> \<Longrightarrow> tsSnd_h\<cdot>(tsLscons\<cdot>(up\<cdot>(uMsg\<cdot>m))\<cdot>msg)\<cdot>(tsLscons\<cdot>(up\<cdot>(uMsg\<cdot>a))\<cdot>acks)\<cdot>ack = 
   (* ack for the current msg \<Longrightarrow> send next msg *)
-  (if (a = ack) then tsMLscons\<cdot>(upApply2 Pair\<cdot>(up\<cdot>m)\<cdot>(up\<cdot>ack))\<cdot>(tsSnd\<cdot>msg\<cdot>acks\<cdot>(Discr (\<not>(undiscr ack))))
+  (if (a = ack) then tsMLscons\<cdot>(upApply2 Pair\<cdot>(up\<cdot>m)\<cdot>(up\<cdot>ack))\<cdot>(tsSnd_h\<cdot>msg\<cdot>acks\<cdot>(Discr (\<not>(undiscr ack))))
   (* wrong ack for the current msg \<Longrightarrow> send msg again *)
-   else tsMLscons\<cdot>(upApply2 Pair\<cdot>(up\<cdot>m)\<cdot>(up\<cdot>ack))\<cdot>(tsSnd\<cdot>(tsMLscons\<cdot>(up\<cdot>m)\<cdot>msg)\<cdot>acks\<cdot>ack))" |
+   else tsMLscons\<cdot>(upApply2 Pair\<cdot>(up\<cdot>m)\<cdot>(up\<cdot>ack))\<cdot>(tsSnd_h\<cdot>(tsMLscons\<cdot>(up\<cdot>m)\<cdot>msg)\<cdot>acks\<cdot>ack))" |
 
   (* if an input and ack is a tick \<Longrightarrow> send msg again plus a tick
-     if transmission starts with tick \<Longrightarrow> #\<surd> acks=\<infinity> *)
-"msg\<noteq>\<bottom> \<Longrightarrow> tsSnd\<cdot>(tsLscons\<cdot>(up\<cdot>(uMsg\<cdot>m))\<cdot>msg)\<cdot>(tsLscons\<cdot>(up\<cdot>DiscrTick)\<cdot>acks)\<cdot>ack 
-  = tsMLscons\<cdot>(upApply2 Pair\<cdot>(up\<cdot>m)\<cdot>(up\<cdot>ack))\<cdot>(delayFun\<cdot>(tsSnd\<cdot>(tsMLscons\<cdot>(up\<cdot>m)\<cdot>msg)\<cdot>acks\<cdot>ack))" |
+     if transmission starts with tick \<Longrightarrow> #\<surd>acks = \<infinity> *)
+"msg \<noteq> \<bottom> \<Longrightarrow> tsSnd_h\<cdot>(tsLscons\<cdot>(up\<cdot>(uMsg\<cdot>m))\<cdot>msg)\<cdot>(tsLscons\<cdot>(up\<cdot>DiscrTick)\<cdot>acks)\<cdot>ack 
+  = tsMLscons\<cdot>(upApply2 Pair\<cdot>(up\<cdot>m)\<cdot>(up\<cdot>ack))\<cdot>(delayFun\<cdot>(tsSnd_h\<cdot>(tsMLscons\<cdot>(up\<cdot>m)\<cdot>msg)\<cdot>acks\<cdot>ack))" |
 
   (* if input is a tick \<Longrightarrow> send tick *)
-"tsSnd\<cdot>(tsLscons\<cdot>(up\<cdot>DiscrTick)\<cdot>msg)\<cdot>(tsLscons\<cdot>(up\<cdot>DiscrTick)\<cdot>acks)\<cdot>ack
-                    = delayFun\<cdot>(tsSnd\<cdot>msg\<cdot>acks\<cdot>ack)" |
+"tsSnd_h\<cdot>(tsLscons\<cdot>(up\<cdot>DiscrTick)\<cdot>msg)\<cdot>(tsLscons\<cdot>(up\<cdot>DiscrTick)\<cdot>acks)\<cdot>ack
+                    = delayFun\<cdot>(tsSnd_h\<cdot>msg\<cdot>acks\<cdot>ack)" |
 
-"acks\<noteq>\<bottom> \<Longrightarrow> tsSnd\<cdot>(tsLscons\<cdot>(up\<cdot>DiscrTick)\<cdot>msg)\<cdot>(tsLscons\<cdot>(up\<cdot>(uMsg\<cdot>a))\<cdot>acks)\<cdot>ack
-                    = delayFun\<cdot>(tsSnd\<cdot>msg\<cdot>(tsMLscons\<cdot>(up\<cdot>a)\<cdot>acks)\<cdot>ack)"
+"acks \<noteq> \<bottom> \<Longrightarrow> tsSnd_h\<cdot>(tsLscons\<cdot>(up\<cdot>DiscrTick)\<cdot>msg)\<cdot>(tsLscons\<cdot>(up\<cdot>(uMsg\<cdot>a))\<cdot>acks)\<cdot>ack
+                    = delayFun\<cdot>(tsSnd_h\<cdot>msg\<cdot>(tsMLscons\<cdot>(up\<cdot>a)\<cdot>acks)\<cdot>ack)"
+
+definition tsSnd :: "'a tstream \<rightarrow> bool tstream \<rightarrow> ('a \<times> bool) tstream" where
+"tsSnd \<equiv> \<Lambda> msg acks. delay (tsSnd_h\<cdot>msg\<cdot>acks\<cdot>(Discr True))"
 
 (* ----------------------------------------------------------------------- *)
 section {* basic properties *}
 (* ----------------------------------------------------------------------- *)
 
-lemma tssnd_strict [simp]:
-"tsSnd\<cdot>\<bottom>\<cdot>\<bottom>\<cdot>ack = \<bottom>"
-"tsSnd\<cdot>\<bottom>\<cdot>acks\<cdot>ack = \<bottom>"
-"tsSnd\<cdot>msg\<cdot>\<bottom>\<cdot>ack = \<bottom>"
+lemma tssnd_insert: "tsSnd\<cdot>msg\<cdot>acks = delay (tsSnd_h\<cdot>msg\<cdot>acks\<cdot>(Discr True))"
+  by (simp add: tsSnd_def)
+
+lemma tssnd_h_strict [simp]:
+"tsSnd_h\<cdot>\<bottom>\<cdot>\<bottom>\<cdot>ack = \<bottom>"
+"tsSnd_h\<cdot>\<bottom>\<cdot>acks\<cdot>ack = \<bottom>"
+"tsSnd_h\<cdot>msg\<cdot>\<bottom>\<cdot>ack = \<bottom>"
   by (fixrec_simp)+
 
-lemma tssnd_delayfun_nack:
-  "msg\<noteq>\<bottom> \<Longrightarrow> tsSnd\<cdot>(tsMLscons\<cdot>(updis m)\<cdot>msg)\<cdot>(delayFun\<cdot>acks)\<cdot>(Discr ack) 
-  = tsMLscons\<cdot>(updis (m, ack))\<cdot>(delayFun\<cdot>(tsSnd\<cdot>(tsMLscons\<cdot>(updis m)\<cdot>msg)\<cdot>acks\<cdot>(Discr ack)))"
-  by (simp add: delayfun_tslscons tsSnd.simps(4) tsmlscons_lscons)
-
-lemma tssnd_delayfun_bot:
-  "msg\<noteq>\<bottom> \<Longrightarrow> tsSnd\<cdot>(tsMLscons\<cdot>(updis m)\<cdot>msg)\<cdot>(delayFun\<cdot>\<bottom>)\<cdot>(Discr ack) 
-     = tsMLscons\<cdot>(updis (m, ack))\<cdot>(delayFun\<cdot>\<bottom>)"
-  by (simp add: tssnd_delayfun_nack)
-
-lemma tssnd_mlscons_ack: "msg\<noteq>\<bottom> \<Longrightarrow> acks\<noteq>\<bottom> \<Longrightarrow>
-   tsSnd\<cdot>(tsMLscons\<cdot>(updis m)\<cdot>msg)\<cdot>(tsMLscons\<cdot>(updis a)\<cdot>acks)\<cdot>(Discr a) 
-     = tsMLscons\<cdot>(updis (m, a))\<cdot>(tsSnd\<cdot>msg\<cdot>acks\<cdot>(Discr (\<not>a)))"
-  by (simp add: tsSnd.simps(3) tsmlscons_lscons)
-
-lemma tssnd_mlscons_nack: "msg\<noteq>\<bottom> \<Longrightarrow> acks\<noteq>\<bottom> \<Longrightarrow> a\<noteq>ack \<Longrightarrow>
-   tsSnd\<cdot>(tsMLscons\<cdot>(updis m)\<cdot>msg)\<cdot>(tsMLscons\<cdot>(updis a)\<cdot>acks)\<cdot>(Discr ack) 
-     = tsMLscons\<cdot>(updis (m, ack))\<cdot>(tsSnd\<cdot>(tsMLscons\<cdot>(updis m)\<cdot>msg)\<cdot>acks\<cdot>(Discr ack))"
-  by (simp add: tsSnd.simps(3) tsmlscons_lscons)
-
-lemma tssnd_delayfun:
-  "tsSnd\<cdot>(delayFun\<cdot>msg)\<cdot>(delayFun\<cdot>acks)\<cdot>ack = delayFun\<cdot>(tsSnd\<cdot>msg\<cdot>acks\<cdot>ack)"
-  by (simp add: delayfun_tslscons tsSnd.simps(5))
-    
-lemma tssnd_delayfun_msg:
-  "acks\<noteq>\<bottom> \<Longrightarrow> tsSnd\<cdot>(delayFun\<cdot>msg)\<cdot>(tsMLscons\<cdot>(updis m)\<cdot>acks)\<cdot>ack 
-                      = delayFun\<cdot>(tsSnd\<cdot>msg\<cdot>(tsMLscons\<cdot>(updis m)\<cdot>acks)\<cdot>ack)"
+lemma tssnd_h_delayfun_nack:
+  "msg \<noteq> \<bottom> \<Longrightarrow> tsSnd_h\<cdot>(tsMLscons\<cdot>(updis m)\<cdot>msg)\<cdot>(delayFun\<cdot>acks)\<cdot>(Discr ack) 
+  = tsMLscons\<cdot>(updis (m, ack))\<cdot>(delayFun\<cdot>(tsSnd_h\<cdot>(tsMLscons\<cdot>(updis m)\<cdot>msg)\<cdot>acks\<cdot>(Discr ack)))"
   by (simp add: delayfun_tslscons tsmlscons_lscons)
 
-(* ToDo: basic properties lemmata for sender *)
+lemma tssnd_h_delayfun_bot:
+  "msg \<noteq> \<bottom> \<Longrightarrow> tsSnd_h\<cdot>(tsMLscons\<cdot>(updis m)\<cdot>msg)\<cdot>(delayFun\<cdot>\<bottom>)\<cdot>(Discr ack) 
+     = tsMLscons\<cdot>(updis (m, ack))\<cdot>(delayFun\<cdot>\<bottom>)"
+  by (simp add: tssnd_h_delayfun_nack)
 
-lemma tssnd_nbot2 [simp]: "msg\<noteq>\<bottom> \<Longrightarrow> tsSnd\<cdot>msg\<cdot>(delayFun\<cdot>acks)\<cdot>(Discr ack) \<noteq> \<bottom>"
+lemma tssnd_h_mlscons_ack: "msg \<noteq> \<bottom> \<Longrightarrow> acks \<noteq> \<bottom> \<Longrightarrow>
+   tsSnd_h\<cdot>(tsMLscons\<cdot>(updis m)\<cdot>msg)\<cdot>(tsMLscons\<cdot>(updis a)\<cdot>acks)\<cdot>(Discr a) 
+     = tsMLscons\<cdot>(updis (m, a))\<cdot>(tsSnd_h\<cdot>msg\<cdot>acks\<cdot>(Discr (\<not>a)))"
+  by (simp add: tsmlscons_lscons)
+
+lemma tssnd_h_mlscons_nack: "msg \<noteq> \<bottom> \<Longrightarrow> acks \<noteq> \<bottom> \<Longrightarrow> a \<noteq> ack \<Longrightarrow>
+   tsSnd_h\<cdot>(tsMLscons\<cdot>(updis m)\<cdot>msg)\<cdot>(tsMLscons\<cdot>(updis a)\<cdot>acks)\<cdot>(Discr ack) 
+     = tsMLscons\<cdot>(updis (m, ack))\<cdot>(tsSnd_h\<cdot>(tsMLscons\<cdot>(updis m)\<cdot>msg)\<cdot>acks\<cdot>(Discr ack))"
+  by (simp add: tsmlscons_lscons)
+
+lemma tssnd_h_delayfun:
+  "tsSnd_h\<cdot>(delayFun\<cdot>msg)\<cdot>(delayFun\<cdot>acks)\<cdot>ack = delayFun\<cdot>(tsSnd_h\<cdot>msg\<cdot>acks\<cdot>ack)"
+  by (simp add: delayfun_tslscons)
+    
+lemma tssnd_h_delayfun_msg:
+  "acks \<noteq> \<bottom> \<Longrightarrow> tsSnd_h\<cdot>(delayFun\<cdot>msg)\<cdot>(tsMLscons\<cdot>(updis m)\<cdot>acks)\<cdot>ack 
+                      = delayFun\<cdot>(tsSnd_h\<cdot>msg\<cdot>(tsMLscons\<cdot>(updis m)\<cdot>acks)\<cdot>ack)"
+  by (simp add: delayfun_tslscons tsmlscons_lscons)
+
+lemma tssnd_h_nbot2 [simp]: "msg \<noteq> \<bottom> \<Longrightarrow> tsSnd_h\<cdot>msg\<cdot>(delayFun\<cdot>acks)\<cdot>(Discr ack) \<noteq> \<bottom>"
   apply (induction msg arbitrary: acks ack)
   apply (simp_all)
   apply (simp add: delayfun_tslscons)
-  by (simp add: tssnd_delayfun_nack)
+  by (simp add: tssnd_h_delayfun_nack)
 
-lemma tssnd_nbot [simp]: "msg\<noteq>\<bottom> \<Longrightarrow> acks\<noteq>\<bottom> \<Longrightarrow> tsSnd\<cdot>msg\<cdot>acks\<cdot>(Discr ack) \<noteq> \<bottom>"
+lemma tssnd_h_nbot [simp]: "msg \<noteq> \<bottom> \<Longrightarrow> acks \<noteq> \<bottom> \<Longrightarrow> tsSnd_h\<cdot>msg\<cdot>acks\<cdot>(Discr ack) \<noteq> \<bottom>"
   apply (induction acks arbitrary: msg ack)
   apply (simp_all)
   apply (rule_tac ts=msg in tscases, simp_all)
   apply (simp add: delayfun_tslscons tsmlscons_lscons)
-  by (smt tsmlscons_bot2 tsmlscons_nbot tssnd_mlscons_ack tssnd_mlscons_nack up_defined)
+  apply (case_tac "t=ack", simp_all)
+  apply (metis tsmlscons_bot2 tsmlscons_nbot tssnd_h_mlscons_ack up_defined)
+  by (metis tsmlscons_bot2 tsmlscons_nbot tssnd_h_mlscons_nack up_defined)
 
-lemma tssnd_tstickcount_adm:
-  "adm (\<lambda>a. \<forall>x. #(Rep_tstream x) \<le> #(Rep_tstream a) \<longrightarrow> (\<forall>xa. #\<surd> x \<le> #\<surd> tsSnd\<cdot>x\<cdot>a\<cdot>(Discr xa)))"
-  apply (rule admI) (* trick adm_imp *)
-  apply (simp add: contlub_cfun_arg contlub_cfun_fun lub_mono2)
+(* ToDo: tstickcount lemma for sender *)
+
+lemma tssnd_h_tstickcount:
+  " min (#\<surd>msg) (#\<surd>acks) \<le> #\<surd> tsSnd_h\<cdot>msg\<cdot>acks\<cdot>(Discr ack)"
   oops
 
-lemma tssnd_tstickcount:
-  "#(Rep_tstream msg) \<le> #(Rep_tstream acks) \<Longrightarrow> #\<surd>msg \<le> #\<surd>(tsSnd\<cdot>msg\<cdot>acks\<cdot>(Discr ack))"
-(*proof (induction msg arbitrary: acks ack, simp_all)
-  case adm
-  then show ?case oops
-next
-  case (delayfun msg)
-  have "Rep_tstream (delay msg) \<noteq> \<epsilon>" oops
-  then show ?case proof (rule tscases [of acks], simp_all)
-    assume "Rep_tstream (delay msg) = \<epsilon>"
-next
-  case (mlscons msg t)
-  then show ?case oops
-qed*)
-(*
-proof (induction acks arbitrary: msg ack)
-  case adm
-  then show ?case
-    apply (rule adm_upward)
-    by (simp add: tssnd_tstickcount_adm) (*proof (rule admI)
-    fix Y :: "nat \<Rightarrow> bool tstream"
-    assume Y_chain: "chain Y"
-    assume a: "\<forall>i x. #(Rep_tstream x) \<le> #(Rep_tstream (Y i)) \<longrightarrow> (\<forall>xa. (#\<surd>x) \<le> (#\<surd>tsSnd\<cdot>x\<cdot>(Y i)\<cdot>(Discr xa)))"
-    assume b: "\<forall>x. #(Rep_tstream x) \<le> #(Rep_tstream (\<Squnion>i. Y i))"
-    from this have "\<forall>x. #(Rep_tstream x) \<le> (\<Squnion>i. #(Rep_tstream (Y i)))" oops
-  qed*)
-next
-  case bottom
-  then show ?case
-    by (simp add: tstickcount_insert)
-next
-  case (delayfun acks)
-  then show ?case proof (rule_tac ts=msg in tscases, simp_all)
-    fix as :: "'a tstream"
-    assume as_leq_acks: "#(Rep_tstream msg) \<le> #(Rep_tstream acks)"
-    assume ind: "(\<And>msg ack. #(Rep_tstream msg) \<le> #(Rep_tstream acks) \<Longrightarrow>
-                 #\<surd>msg \<le> #\<surd> tsSnd\<cdot>msg\<cdot>acks\<cdot>(Discr ack))"
-    hence "#\<surd>msg \<le> #\<surd> tsSnd\<cdot>msg\<cdot>acks\<cdot>(Discr ack)"
-      using as_leq_acks by (simp add: delayfun.IH)
-    have "#\<surd> delay as = lnsuc\<cdot>(#\<surd>as)" by (simp add: delayFun_def)
-    have "tsSnd\<cdot>(delay as)\<cdot>(delay acks)\<cdot>(Discr ack) = delay (tsSnd\<cdot>as\<cdot>acks\<cdot>(Discr ack))"
-      by (simp add: tsSnd.simps(5) delayfun_tslscons)
-    oops
-next
-  case (mlscons acks t)
-  then show ?case oops
-*)
-oops
-
-lemma tssnd_tsabs_slen:
-  "#(Rep_tstream msg) \<le> #(Rep_tstream acks) \<Longrightarrow> #(tsAbs\<cdot>msg) \<le> #(tsAbs\<cdot>(tsSnd\<cdot>msg\<cdot>acks\<cdot>ack))"
-oops
-
-lemma tssnd_inftick: "acks\<noteq>\<bottom> \<Longrightarrow> tsSnd\<cdot>tsInfTick\<cdot>acks\<cdot>ack = tsInfTick"
-proof (induction acks arbitrary: ack)
-  case adm
-  then show ?case by (rule adm_imp, simp_all)
-next
-  case bottom
-  then show ?case using bottom.prems by blast
-next
-  case (delayfun acks)
-  (*have delay_inftick: "delay (Abs_tstream \<up>(\<surd>::'a event)\<infinity>) = tsInfTick"
-    by (metis (no_types)
-        Rep_Abs delayFun.rep_eq sinftimes_unfold tick_msg tsInfTick.abs_eq tsInfTick.rep_eq
-        tsconc_insert)*)
-  have inftick_delay: "tsInfTick = delay tsInfTick" by simp
-  have delay_both: "\<forall>msg acks' ack'. acks' = \<bottom> \<or>
-        tsSnd\<cdot>(delay (msg::'a tstream))\<cdot>(delay (acks'::bool tstream))\<cdot>ack' = delay (tsSnd\<cdot>msg\<cdot>acks'\<cdot>ack')"
-    using tssnd_delayfun by blast
-  assume ind: "\<And>ack. acks \<noteq> \<bottom> \<Longrightarrow> tsSnd\<cdot>tsInfTick\<cdot>acks\<cdot>ack = tsInfTick"
-  have delay_nbot: "delay acks \<noteq> \<bottom>" by simp
-  show ?case
-    apply (subst inftick_delay)
-    (*apply (case_tac "acks = \<bottom>", simp_all)*)
-    apply (subst tssnd_delayfun)
-    sorry
-next
-  case (mlscons acks t)
-  have inftick_delay: "tsInfTick = delay tsInfTick" by simp
-  have delay_msg: "\<forall>msg acks' ack1' ack2'. acks' = \<bottom> \<or>
-        tsSnd\<cdot>(delay (msg::'a tstream))\<cdot>(tsMLscons\<cdot>(updis (ack1'::bool))\<cdot>(acks'::bool tstream))\<cdot>ack2' =
-        delay (tsSnd\<cdot>msg\<cdot>(tsMLscons\<cdot>(updis ack1')\<cdot>acks')\<cdot>ack2')"
-    by (metis delayfun_tslscons tsSnd.simps(6) tsmlscons_lscons)
-  show ?case
-    by (smt delayFun.rep_eq delay_msg inftick_delay mlscons.hyps s2sinftimes tick_msg tsconc_insert
-            tsconc_rep_eq)
-oops
+lemma tssnd_h_inftick_inftick: "tsSnd_h\<cdot>tsInfTick\<cdot>tsInfTick\<cdot>ack = tsInfTick" 
+  by (metis (no_types, lifting) Rep_Abs delayfun_insert s2sinftimes sinftimes_unfold tick_msg 
+      tsInfTick.rep_eq tsInfTick_def tsconc_insert tsconc_rep_eq tssnd_h_delayfun)
 
 (* ----------------------------------------------------------------------- *)
 section {* additional properties *}
 (* ----------------------------------------------------------------------- *)
 
+text {* lemmata for sender, see BS01, page 103 
+   fds = stream of transmitted messages
+   fb = corresponding stream of bits
+   fas = stream of received acknowledgments
+   i = input stream
+   as = acks stream
+   ds = output stream
+*}
+
 (* ToDo: additional properties lemmata for sender *)
 
-lemma tssnd_inftick_inftick: "tsSnd\<cdot>tsInfTick\<cdot>tsInfTick\<cdot>ack = tsInfTick" 
-  by (metis (no_types, lifting) Rep_Abs delayfun_insert s2sinftimes sinftimes_unfold tick_msg 
-      tsInfTick.rep_eq tsInfTick_def tsconc_insert tsconc_rep_eq tssnd_delayfun)
-  
-lemma tssnd_delayfun_abs:
-  "tsAbs\<cdot>(tsSnd\<cdot>(delayFun\<cdot>msg)\<cdot>(delayFun\<cdot>acks)\<cdot>ack) 
-                      = tsAbs\<cdot>(tsSnd\<cdot>msg\<cdot>acks\<cdot>ack)"
-  by (simp add: tssnd_delayfun)
-
-lemma tssnd_delayfun_nack_abs:
-  "msg\<noteq>\<bottom> \<Longrightarrow> tsAbs\<cdot>(tsSnd\<cdot>(tsMLscons\<cdot>(updis m)\<cdot>msg)\<cdot>(delayFun\<cdot>acks)\<cdot>(Discr ack)) 
-  = updis (m, ack) && (tsAbs\<cdot>(tsSnd\<cdot>(tsMLscons\<cdot>(updis m)\<cdot>msg)\<cdot>acks\<cdot>(Discr ack)))"
-  by (simp add: tssnd_delayfun_nack tsabs_mlscons)
-
-lemma tssnd_delayfun_bot_abs:
-  "msg\<noteq>\<bottom> \<Longrightarrow> tsAbs\<cdot>(tsSnd\<cdot>(tsMLscons\<cdot>(updis m)\<cdot>msg)\<cdot>(delayFun\<cdot>\<bottom>)\<cdot>(Discr ack)) 
-     = updis (m, ack) && \<bottom>"
-  by (simp add: tssnd_delayfun_bot tsabs_mlscons)
-
-lemma tssnd_mlscons_nack_abs: "msg\<noteq>\<bottom> \<Longrightarrow> acks\<noteq>\<bottom> \<Longrightarrow> a\<noteq>ack \<Longrightarrow>
-   tsAbs\<cdot>(tsSnd\<cdot>(tsMLscons\<cdot>(updis m)\<cdot>msg)\<cdot>(tsMLscons\<cdot>(updis a)\<cdot>acks)\<cdot>(Discr ack)) 
-     = updis (m, ack) && tsAbs\<cdot>(tsSnd\<cdot>(tsMLscons\<cdot>(updis m)\<cdot>msg)\<cdot>acks\<cdot>(Discr ack))"
-  by (simp add: tssnd_mlscons_nack tsabs_mlscons)
-    
-lemma tssnd_delayfun_msg_abs:
-  "acks\<noteq>\<bottom> \<Longrightarrow> tsAbs\<cdot>(tsSnd\<cdot>(delayFun\<cdot>msg)\<cdot>(tsMLscons\<cdot>(updis m)\<cdot>acks)\<cdot>ack) 
-                      = tsAbs\<cdot>(tsSnd\<cdot>msg\<cdot>(tsMLscons\<cdot>(updis m)\<cdot>acks)\<cdot>ack)"
-  by(simp add: tssnd_delayfun_msg)
-    
-lemma tssnd_mlscons_ack_abs:"msg\<noteq>\<bottom> \<Longrightarrow> acks\<noteq>\<bottom> \<Longrightarrow>
-   tsAbs\<cdot>((tsSnd\<cdot>(tsMLscons\<cdot>(updis m)\<cdot>msg)\<cdot>(tsMLscons\<cdot>(updis a)\<cdot>acks)\<cdot>(Discr a))) 
-     = (updis (m, a)) && (tsAbs\<cdot>(tsSnd\<cdot>msg\<cdot>acks\<cdot>(Discr (\<not>a))))"
-  by (simp add: tsabs_mlscons tssnd_mlscons_ack)
-
-
 text {* fds \<sqsubseteq> i where fds = map(\<alpha>.ds, \<Pi>1) 
-        fds is a prefix of i *} 
-
-lemma tssnd_prefix_inp_h4:"(\<And>tb ack as. sprojfst\<cdot>(srcdups\<cdot>(\<up>(tb, ack) \<bullet> 
-          tsAbs\<cdot>(tsSnd\<cdot>asc\<cdot>as\<cdot>(Discr (\<not> ack))))) \<sqsubseteq>\<up>tb \<bullet> tsAbs\<cdot>asc) \<Longrightarrow>\<up>ta \<bullet> 
-          sprojfst\<cdot>(srcdups\<cdot>(\<up>(tb, \<not> ack) \<bullet> tsAbs\<cdot>(tsSnd\<cdot>asc\<cdot>as\<cdot>(Discr ack)))) \<sqsubseteq> \<up>ta \<bullet> \<up>tb \<bullet> tsAbs\<cdot>asc"
-  proof(induction as arbitrary: ta tb ack asc)
-    case adm
-    then show ?case
-    by(simp)  
-  next
-    case bottom
-    then show ?case
-    by(simp add: monofun_cfun_arg)  
-  next
-    case (delayfun as)
-    then show ?case
-      apply(rule_tac ts = asc in tscases, simp_all)
-      apply(simp add: tssnd_delayfun_abs)
-      apply (metis tssnd_delayfun_abs)
-      apply (case_tac "as = \<bottom>", simp_all)
-      apply(simp add: tssnd_delayfun_nack_abs lscons_conv tsabs_mlscons)
-    proof -
-      fix a :: 'a and asb :: "'a tstream"
-      assume a1: "\<And>tb ack as. sprojfst\<cdot> (srcdups\<cdot> (\<up>(tb, ack) \<bullet> 
-               tsAbs\<cdot> (tsSnd\<cdot> (tsMLscons\<cdot>(updis a)\<cdot>asb)\<cdot> as\<cdot> (Discr (\<not> ack))))) \<sqsubseteq> \<up>tb \<bullet> \<up>a \<bullet> tsAbs\<cdot>asb"
-      assume a2: "asb \<noteq> \<bottom>"
-      have "ack = ack"
-        by auto
-      then have f0:"\<And> ack. sprojfst\<cdot> (srcdups\<cdot> (\<up>(a,  ack) \<bullet> 
-     tsAbs\<cdot> (tsSnd\<cdot> (tsMLscons\<cdot>(updis a)\<cdot> asb)\<cdot> (delayFun\<cdot>as)\<cdot> (Discr (\<not> ack))))) \<sqsubseteq> \<up>a \<bullet> \<up>a \<bullet> tsAbs\<cdot>asb"
-        using a1 by auto
-      then have f3: "sprojfst\<cdot> (srcdups\<cdot> (\<up>(a, \<not> ack) \<bullet> 
-         tsAbs\<cdot> (tsSnd\<cdot> (tsMLscons\<cdot>(updis a)\<cdot> asb)\<cdot> (delayFun\<cdot>as)\<cdot> (Discr ack)))) \<sqsubseteq> \<up>a \<bullet> \<up>a \<bullet> tsAbs\<cdot>asb"
-        by (insert f0 [of "\<not>ack"], auto)
-      have "tsAbs\<cdot> (tsSnd\<cdot>(tsMLscons\<cdot>(updis a)\<cdot>asb)\<cdot> (delayFun\<cdot>as)\<cdot> (Discr ack)) = updis (a, ack) && 
-          tsAbs\<cdot> (tsSnd\<cdot>(tsMLscons\<cdot>(updis a)\<cdot>asb)\<cdot>as\<cdot> (Discr ack))"
-        using a2 by (meson tssnd_delayfun_nack_abs)
-      then have "srcdups\<cdot> (\<up>(a, \<not> ack) \<bullet> tsAbs\<cdot> (tsSnd\<cdot> (tsMLscons\<cdot>(updis a)\<cdot> asb)\<cdot> (delayFun\<cdot>as)\<cdot> 
-                                   (Discr ack))) = \<up>(a, \<not> ack) \<bullet> srcdups\<cdot> (\<up>(a, ack) \<bullet> 
-                                  tsAbs\<cdot> (tsSnd\<cdot>(tsMLscons\<cdot>(updis a)\<cdot>asb)\<cdot> as\<cdot> (Discr ack)))"
-        by (simp add: lscons_conv)
-      then have "\<up>a \<bullet> sprojfst\<cdot> (srcdups\<cdot> (\<up>(a, ack) \<bullet> tsAbs\<cdot> 
-                          (tsSnd\<cdot>(tsMLscons\<cdot>(updis a)\<cdot>asb)\<cdot>as\<cdot> (Discr ack)))) \<sqsubseteq> \<up>a \<bullet> \<up>a \<bullet> tsAbs\<cdot>asb"
-        using f3 by simp
-      then show "\<up>ta \<bullet> \<up>tb \<bullet> sprojfst\<cdot> (srcdups\<cdot> (\<up>(a, ack) \<bullet> 
-              tsAbs\<cdot> (tsSnd\<cdot> (tsMLscons\<cdot>(updis a)\<cdot>asb)\<cdot> as\<cdot> (Discr ack)))) \<sqsubseteq> \<up>ta \<bullet> \<up>tb \<bullet> \<up>a \<bullet> tsAbs\<cdot>asb"
-        by (meson less_all_sconsD monofun_cfun_arg)
-    qed
-  next
-    case (mlscons asa t)
-    then show ?case
-    apply(rule_tac ts = asc in tscases, simp_all)
-    apply(simp add: tssnd_delayfun_msg_abs)defer
-    apply(case_tac "as=\<bottom>", simp_all)
-    apply(case_tac "t= ack", simp_all)
-    apply(simp add: tssnd_mlscons_ack_abs lscons_conv tsabs_mlscons)defer
-    apply(simp add: tssnd_mlscons_nack_abs lscons_conv tsabs_mlscons)
-    proof -
-      fix a :: 'a and as :: "'a tstream" and asa :: "bool tstream"
-      assume a1: "\<And>tb ack asa. sprojfst\<cdot> (srcdups\<cdot> (\<up>(tb, ack) \<bullet> 
-                tsAbs\<cdot> (tsSnd\<cdot> (tsMLscons\<cdot>(updis a)\<cdot>as)\<cdot> asa\<cdot> (Discr (\<not> ack))))) \<sqsubseteq> \<up>tb \<bullet> \<up>a \<bullet> tsAbs\<cdot>as"
-      assume a2: "asa \<noteq> \<bottom>"
-      assume a3: "as \<noteq> \<bottom>"
-      have "ack = ack"
-        by auto
-      then have f0: "\<And>ack asa. sprojfst\<cdot> (srcdups\<cdot> (\<up>(tb,  ack) \<bullet> 
-                tsAbs\<cdot> (tsSnd\<cdot> (tsMLscons\<cdot>(updis a)\<cdot> as)\<cdot> asa\<cdot> (Discr (\<not>ack))))) \<sqsubseteq> \<up>tb \<bullet> \<up>a \<bullet> tsAbs\<cdot>as"
-        using a1 by blast
-      then have "sprojfst\<cdot> (srcdups\<cdot> (\<up>(tb, \<not> ack) \<bullet> tsAbs\<cdot> (tsSnd\<cdot> (tsMLscons\<cdot>(updis a)\<cdot> as)\<cdot> 
-                                     (tsMLscons\<cdot>(updis ack)\<cdot>asa)\<cdot>(Discr ack)))) \<sqsubseteq> \<up>tb \<bullet> \<up>a \<bullet> tsAbs\<cdot>as"
-        by (insert f0 [of "\<not>ack"], auto)
-      then have "\<up>tb \<bullet> sprojfst\<cdot> (srcdups\<cdot> ( \<up>(a,  ack) \<bullet> tsAbs\<cdot> (tsSnd\<cdot>as\<cdot>asa\<cdot>(Discr (\<not> ack))))) 
-                 \<sqsubseteq> \<up>tb \<bullet> \<up>a \<bullet> tsAbs\<cdot>as"
-        by (simp add: a2 a3 lscons_conv tssnd_mlscons_ack_abs)
-      then show "\<up>ta \<bullet> \<up>tb \<bullet> sprojfst\<cdot>(srcdups\<cdot>(\<up>(a, ack) \<bullet> tsAbs\<cdot>(tsSnd\<cdot>as\<cdot>asa\<cdot>(Discr (\<not> ack))))) 
-                    \<sqsubseteq> \<up>ta \<bullet> \<up>tb \<bullet> \<up>a \<bullet> tsAbs\<cdot>as"
-        using monofun_cfun_arg by blast
-    next
-      fix a :: 'a and asb :: "'a tstream"
-      assume a1: "\<And>tb ack as. sprojfst\<cdot> (srcdups\<cdot> (\<up>(tb, ack) \<bullet> tsAbs\<cdot> 
-                      (tsSnd\<cdot> (tsMLscons\<cdot>(updis a)\<cdot>asb)\<cdot> as\<cdot> (Discr (\<not> ack))))) \<sqsubseteq> \<up>tb \<bullet> \<up>a \<bullet> tsAbs\<cdot>asb"
-      assume a2: "asb \<noteq> \<bottom>"
-      have "ack = ack"
-        by auto
-      then have f0:"\<And>ack. sprojfst\<cdot> (srcdups\<cdot> (\<up>(a,  ack) \<bullet> tsAbs\<cdot> (tsSnd\<cdot> (tsMLscons\<cdot>(updis a)\<cdot> asb)\<cdot> 
-                        (delayFun\<cdot>asa)\<cdot> (Discr (\<not> ack))))) \<sqsubseteq> \<up>a \<bullet> \<up>a \<bullet> tsAbs\<cdot>asb"
-        using a1 by blast
-      then have "sprojfst\<cdot> (srcdups\<cdot> (\<up>(a, \<not> ack) \<bullet> tsAbs\<cdot> (tsSnd\<cdot> (tsMLscons\<cdot>(updis a)\<cdot> asb)\<cdot> 
-                 (delayFun\<cdot>asa)\<cdot> (Discr ack)))) \<sqsubseteq> \<up>a \<bullet> \<up>a \<bullet> tsAbs\<cdot>asb"
-        by (insert f0 [of "\<not>ack"], auto) 
-      then have "\<up>a \<bullet> sprojfst\<cdot> (srcdups\<cdot> (\<up>(a, ack) \<bullet> tsAbs\<cdot> (tsSnd\<cdot>(tsMLscons\<cdot>(updis a)\<cdot>asb)\<cdot>asa\<cdot> 
-                   (Discr ack)))) \<sqsubseteq> \<up>a \<bullet> \<up>a \<bullet> tsAbs\<cdot>asb"
-        using a2 by (simp add: lscons_conv tssnd_delayfun_nack_abs)
-      then show "\<up>ta \<bullet> \<up>tb \<bullet> sprojfst\<cdot> (srcdups\<cdot> (\<up>(a, ack) \<bullet> tsAbs\<cdot> (tsSnd\<cdot> (tsMLscons\<cdot>(updis a)\<cdot>asb)\<cdot> 
-                asa\<cdot> (Discr ack)))) \<sqsubseteq> \<up>ta \<bullet> \<up>tb \<bullet> \<up>a \<bullet> tsAbs\<cdot>asb"
-        by (meson less_all_sconsD monofun_cfun_arg)
-    next
-      fix asb :: "'a tstream"
-      assume a1: "\<And>tb ack as. sprojfst\<cdot> (srcdups\<cdot> (\<up>(tb, ack) \<bullet> tsAbs\<cdot> (tsSnd\<cdot>(delayFun\<cdot>asb)\<cdot>as\<cdot> 
-                    (Discr (\<not> ack))))) \<sqsubseteq> \<up>tb \<bullet> tsAbs\<cdot>asb"
-      have "ack = ack"
-        by auto
-      then have f0: "\<And>ack . sprojfst\<cdot> (srcdups\<cdot> (\<up>(tb, ack) \<bullet> tsAbs\<cdot> (tsSnd\<cdot>(delayFun\<cdot>asb)\<cdot>(delayFun\<cdot> 
-                    (tsMLscons\<cdot>(updis t)\<cdot> asa))\<cdot> (Discr (\<not> ack))))) \<sqsubseteq> \<up>tb \<bullet> tsAbs\<cdot>asb"
-        using a1 by auto
-      then have "sprojfst\<cdot> (srcdups\<cdot> (\<up>(tb, \<not> ack) \<bullet> tsAbs\<cdot> (tsSnd\<cdot>(delayFun\<cdot>asb)\<cdot> 
-                        (delayFun\<cdot> (tsMLscons\<cdot>(updis t)\<cdot> asa))\<cdot> (Discr ack)))) \<sqsubseteq> \<up>tb \<bullet> tsAbs\<cdot>asb"
-        by (insert f0 [of "\<not>ack"], auto)
-      then show "\<up>ta \<bullet> sprojfst\<cdot> (srcdups\<cdot> (\<up>(tb, \<not> ack) \<bullet> tsAbs\<cdot> (tsSnd\<cdot>asb\<cdot> (tsMLscons\<cdot>(updis t)\<cdot>asa)\<cdot> 
-                   (Discr ack)))) \<sqsubseteq> \<up>ta \<bullet> \<up>tb \<bullet> tsAbs\<cdot>asb"
-        by (simp add: monofun_cfun_arg tsabs_delayfun tssnd_delayfun)
-    qed
-  qed
-
-lemma tssnd_prefix_inp_h3:"(\<And>ta ack as. sprojfst\<cdot>(srcdups\<cdot>(\<up>(ta, ack) \<bullet> tsAbs\<cdot>(tsSnd\<cdot>asa\<cdot>as\<cdot>
-           (Discr (\<not> ack))))) \<sqsubseteq> \<up>ta \<bullet> tsAbs\<cdot>asa) \<Longrightarrow> asa \<noteq> \<bottom> \<Longrightarrow> \<up>ta \<bullet> sprojfst\<cdot>(srcdups\<cdot>(\<up>(t, \<not> ack)
-            \<bullet> tsAbs\<cdot>(tsSnd\<cdot>(tsMLscons\<cdot>(updis t)\<cdot>asa)\<cdot>as\<cdot>(Discr (\<not> ack))))) \<sqsubseteq> \<up>ta \<bullet> \<up>t \<bullet> tsAbs\<cdot>asa"
-  apply(induction as arbitrary: ta t ack asa,simp_all)
-  apply(simp add: monofun_cfun_arg)
-  apply(simp add: tssnd_delayfun_nack_abs lscons_conv)
-  apply(case_tac "t=ack")
-  apply(simp add: tssnd_mlscons_nack_abs lscons_conv)
-  by(simp add: tssnd_mlscons_ack_abs lscons_conv tssnd_prefix_inp_h4)  
-    
-lemma tssnd_prefix_inp_h2:"sprojfst\<cdot>(srcdups\<cdot>(updis (ta, ack) && tsAbs\<cdot>(tsSnd\<cdot>asc\<cdot>as\<cdot>(Discr (\<not> ack)))))
-                         \<sqsubseteq> updis ta && tsAbs\<cdot>asc"
-  proof(induction asc arbitrary: ta ack as)
-  fix asc:: "'a tstream" and as:: "bool tstream" and ack:: "bool discr" and ta:: "'a"
-    case adm
-    then show ?case 
-    by simp
-  next
-    case bottom
-    then show ?case
-    by(simp add: lscons_conv)
-  next
-    case (delayfun asa)
-    then show ?case
-    apply(rule_tac ts = as in tscases, simp_all)
-    apply(simp add: lscons_conv)    
-    apply(simp add: tssnd_delayfun_abs)
-    apply(case_tac "as=\<bottom>")    
-    apply(simp add: lscons_conv)    
-    by(simp add: tssnd_delayfun_msg_abs)
-  next
-    case (mlscons asa t)
-    then show ?case
-    apply(rule_tac ts=as in tscases, simp_all)
-    apply(simp add: lscons_conv)  
-    apply(simp add: tssnd_delayfun_nack_abs lscons_conv tsabs_mlscons tssnd_prefix_inp_h3)
-    apply(case_tac "as=\<bottom>",simp)
-    apply(simp add:lscons_conv)
-    apply(case_tac "a=ack")
-    apply(simp add: tssnd_mlscons_nack_abs tsabs_mlscons lscons_conv tssnd_prefix_inp_h3) 
-    apply(simp add: tssnd_mlscons_ack_abs lscons_conv tsabs_mlscons)
-    proof -
-      fix a :: bool and asd :: "bool tstream"
-      assume a1: "\<And>ta ack as. sprojfst\<cdot> (srcdups\<cdot> (\<up>(ta, ack) \<bullet> tsAbs\<cdot> (tsSnd\<cdot>asa\<cdot>as\<cdot> 
-                    (Discr (\<not> ack))))) \<sqsubseteq> \<up>ta \<bullet> tsAbs\<cdot>asa"
-      have "ack = ack"
-        by auto
-      then have f0: "\<And>ack . sprojfst\<cdot> (srcdups\<cdot> (\<up>(t, ack) \<bullet> tsAbs\<cdot> (tsSnd\<cdot>asa\<cdot>asd\<cdot> (Discr (\<not> ack))))) 
-                   \<sqsubseteq> \<up>t \<bullet> tsAbs\<cdot>asa"
-        using a1 by auto    
-      then have "sprojfst\<cdot> (srcdups\<cdot> (\<up>(t, \<not> ack) \<bullet> tsAbs\<cdot> (tsSnd\<cdot>asa\<cdot>asd\<cdot> (Discr ack)))) 
-                \<sqsubseteq> \<up>t \<bullet> tsAbs\<cdot>asa"
-        by (insert f0 [of "\<not>ack"], auto)
-      then show "\<up>ta \<bullet> sprojfst\<cdot> (srcdups\<cdot> (\<up>(t, \<not> ack) \<bullet> tsAbs\<cdot> (tsSnd\<cdot>asa\<cdot>asd\<cdot>(Discr ack)))) 
-              \<sqsubseteq> \<up>ta \<bullet> \<up>t \<bullet> tsAbs\<cdot>asa"
-        using monofun_cfun_arg by blast
-      qed
-  qed
-    
-lemma tssnd_prefix_inp_h1: "asc \<noteq> \<bottom> \<Longrightarrow>
-    sprojfst\<cdot>
-    (srcdups\<cdot>( \<up>(t, ack) \<bullet> tsAbs\<cdot>(tsSnd\<cdot>(tsMLscons\<cdot>(updis t)\<cdot>asc)\<cdot>as\<cdot>(Discr ack)))) \<sqsubseteq>
-    \<up>t \<bullet> tsAbs\<cdot>asc"
-  apply(induction as arbitrary: t ack asc, simp_all)
-  apply(simp add: tssnd_delayfun_nack_abs lscons_conv)
-  apply(case_tac "t\<noteq>ack")
-  apply(simp add: tssnd_mlscons_nack_abs lscons_conv)
-  apply(simp add: tssnd_mlscons_ack tsabs_mlscons lscons_conv)
-  by (metis lscons_conv tssnd_prefix_inp_h2)
-
-lemma tssnd_prefix_inp: "tsAbs\<cdot>(tsProjFst\<cdot>(tsRemDups\<cdot>(tsSnd\<cdot>i\<cdot>as\<cdot>(Discr ack)))) \<sqsubseteq> tsAbs\<cdot>i"
-  apply(simp add: tsremdups_tsabs tsprojfst_tsabs)
-  proof(induction as arbitrary: i ack,simp_all)
-    fix i:: "'a tstream" and as:: "bool tstream" and ack:: "bool discr"
-    case (delayfun as)
-    then show ?case
-    apply(rule_tac ts = i in tscases, simp_all)
-    apply(simp add: tssnd_delayfun_abs)
-    apply(case_tac "as=\<bottom>")    
-    apply(simp add: lscons_conv)    
-    by(simp add: tssnd_delayfun_nack_abs lscons_conv tsabs_mlscons tssnd_prefix_inp_h1)
-  next
-    case (mlscons as t)
-    then show ?case
-    proof(induction i arbitrary: t as ack)
-      case adm
-      then show ?case by simp
-    next
-      case bottom
-      then show ?case by simp
-    next
-      case (delayfun i)
-      then show ?case
-      by(simp add: tssnd_delayfun_msg_abs)
-    next
-      case (mlscons i ta)
-      then show ?case
-      apply(case_tac "t\<noteq>ack")
-      apply(simp add: tssnd_mlscons_nack_abs tsabs_mlscons lscons_conv tssnd_prefix_inp_h1)
-      by(simp add: tssnd_mlscons_ack tsabs_mlscons tssnd_prefix_inp_h2)
-    qed
-  qed
-    
+        fds is a prefix of i *}
+lemma tssnd_prefix_inp: "tsAbs\<cdot>(tsProjFst\<cdot>(tsRemDups\<cdot>(tsSnd_h\<cdot>i\<cdot>as\<cdot>(Discr ack)))) \<sqsubseteq> tsAbs\<cdot>i"
+  oops
     
 text {* \<alpha>.fb = fb  where fb = map(\<alpha>.ds, \<Pi>2)
         each new data element from i is assigned a bit different from the bit assigned to 
         the previous one*}
-lemma tssnd_alt_bit_h5:"(\<And>ack t as. srcdups\<cdot>(\<up>ack \<bullet> sprojsnd\<cdot>(srcdups\<cdot>(\<up>(t, \<not> ack) \<bullet> 
-      tsAbs\<cdot>(tsSnd\<cdot>asa\<cdot>as\<cdot>(Discr ack))))) = \<up>ack \<bullet> sprojsnd\<cdot>(srcdups\<cdot>(\<up>(t, \<not> ack) \<bullet> tsAbs\<cdot>(tsSnd\<cdot>asa\<cdot>as\<cdot>
- (Discr ack))))) \<Longrightarrow> asa\<noteq>\<bottom> \<Longrightarrow> \<up>ack \<bullet> srcdups\<cdot>(\<up>(\<not> ack) \<bullet> sprojsnd\<cdot>(srcdups\<cdot>(\<up>(ta, ack) \<bullet> 
-  tsAbs\<cdot>(tsSnd\<cdot>(tsMLscons\<cdot>(updis ta)\<cdot>asa)\<cdot>as\<cdot>(Discr ack))))) = \<up>ack \<bullet> \<up>(\<not> ack) \<bullet> 
-    sprojsnd\<cdot>(srcdups\<cdot>(\<up>(ta, ack) \<bullet> tsAbs\<cdot>(tsSnd\<cdot>(tsMLscons\<cdot>(updis ta)\<cdot>asa)\<cdot>as\<cdot>(Discr ack))))"
-  apply(induction as arbitrary: ta ack asa,simp_all)
-  apply(subst srcdups_def [THEN fix_eq2],simp)
-  apply(simp add: tssnd_delayfun_nack_abs lscons_conv)
-  apply(case_tac "t\<noteq>ack")
-  apply(simp add: tssnd_mlscons_nack_abs lscons_conv)
-  apply(simp add: tssnd_mlscons_ack_abs lscons_conv)
-  proof -
-    fix asb :: "bool tstream" and t :: bool and taa :: 'a and acka :: bool and asaa :: "'a tstream"
-    assume a1: "\<And>ack t as. srcdups\<cdot> (\<up>ack \<bullet> sprojsnd\<cdot> (srcdups\<cdot> (\<up>(t, \<not> ack) \<bullet> tsAbs\<cdot> (tsSnd\<cdot>asaa\<cdot>as\<cdot>
-      (Discr ack))))) = \<up>ack \<bullet> sprojsnd\<cdot> (srcdups\<cdot> (\<up>(t, \<not> ack) \<bullet> tsAbs\<cdot> (tsSnd\<cdot>asaa\<cdot>as\<cdot>(Discr ack))))"
-    then have f0:"\<And>ack. srcdups\<cdot> (\<up>ack \<bullet> sprojsnd\<cdot> (srcdups\<cdot> (\<up>(taa, \<not> ack) \<bullet> tsAbs\<cdot> (tsSnd\<cdot>asaa\<cdot>asb\<cdot>
-   (Discr ack))))) = \<up>ack \<bullet> sprojsnd\<cdot> (srcdups\<cdot> (\<up>(taa, \<not> ack) \<bullet> tsAbs\<cdot> (tsSnd\<cdot>asaa\<cdot>asb\<cdot>(Discr ack))))"
-      by auto
-    then have"srcdups\<cdot> (\<up>(\<not> acka) \<bullet> sprojsnd\<cdot> (srcdups\<cdot> (\<up>(taa, acka) \<bullet> tsAbs\<cdot> (tsSnd\<cdot>asaa\<cdot>asb\<cdot> 
-       (Discr (\<not> acka)))))) = \<up>(\<not> acka) \<bullet> sprojsnd\<cdot> (srcdups\<cdot> (\<up>(taa, acka) \<bullet> tsAbs\<cdot> (tsSnd\<cdot>asaa\<cdot>asb\<cdot> 
-            (Discr (\<not> acka)))))"
-      by (insert f0 [of "\<not>acka"], auto)
-    then show "\<up>acka \<bullet> srcdups\<cdot> (\<up>(\<not> acka) \<bullet> sprojsnd\<cdot> (srcdups\<cdot> (\<up>(taa, acka) \<bullet> tsAbs\<cdot>(tsSnd\<cdot>asaa\<cdot>asb\<cdot>
-   (Discr (\<not> acka)))))) = \<up>acka \<bullet> \<up>(\<not> acka) \<bullet> sprojsnd\<cdot>(srcdups\<cdot> (\<up>(taa, acka) \<bullet> tsAbs\<cdot>(tsSnd\<cdot>asaa\<cdot>asb\<cdot> 
-             (Discr (\<not> acka)))))"
-      by simp
-  qed
-
-lemma tssnd_alt_bit_h4:
-          "srcdups\<cdot>(\<up>ack \<bullet> sprojsnd\<cdot>(srcdups\<cdot>(\<up>(t, \<not> ack) \<bullet> tsAbs\<cdot>(tsSnd\<cdot>i\<cdot>as\<cdot>(Discr ack))))) 
-                          = \<up>ack \<bullet> sprojsnd\<cdot>(srcdups\<cdot>(\<up>(t, \<not> ack) \<bullet> tsAbs\<cdot>(tsSnd\<cdot>i\<cdot>as\<cdot>(Discr ack))))"
-  proof(induction i arbitrary: ack t as)
-  fix i:: "'a tstream" and as:: "bool tstream" and ack:: "bool discr" and t::"'a"
-    case adm
-    then show ?case
-    by simp
-  next
-    case bottom
-    then show ?case 
-    by(subst srcdups_def [THEN fix_eq2],simp)
-  next
-    case (delayfun asa)
-    then show ?case
-      apply(rule_tac ts= as in tscases, simp_all)
-      apply(subst srcdups_def [THEN fix_eq2],simp)
-      apply(simp add: tssnd_delayfun_abs)
-      apply(case_tac "as=\<bottom>", simp_all)
-      apply(subst srcdups_def [THEN fix_eq2],simp)
-      by(simp add: tssnd_delayfun_msg_abs)
-  next
-    case (mlscons asa ta)
-    then show ?case
-    apply(rule_tac ts= as in tscases, simp_all)
-    apply(subst srcdups_def [THEN fix_eq2],simp)
-    apply(simp add: tssnd_delayfun_nack_abs lscons_conv tssnd_alt_bit_h5)
-    apply(case_tac "as=\<bottom>", simp)
-    apply(subst srcdups_def [THEN fix_eq2],simp_all)
-    apply(case_tac "a\<noteq>ack", simp_all)
-    apply(simp add: tssnd_mlscons_nack_abs lscons_conv tssnd_alt_bit_h5)    
-    apply(simp add: tssnd_mlscons_ack_abs lscons_conv)
-    proof -
-      fix a :: bool and asc :: "bool tstream"
-      assume a1: "\<And>ack t as. srcdups\<cdot> (\<up>ack \<bullet> sprojsnd\<cdot> (srcdups\<cdot> (\<up>(t, \<not> ack) \<bullet> tsAbs\<cdot> (tsSnd\<cdot>asa\<cdot>as\<cdot>
-       (Discr ack))))) = \<up>ack \<bullet> sprojsnd\<cdot> (srcdups\<cdot> (\<up>(t, \<not> ack) \<bullet> tsAbs\<cdot> (tsSnd\<cdot>asa\<cdot>as\<cdot>(Discr ack))))"
-      then have f0:"\<And>ack. srcdups\<cdot> (\<up>ack \<bullet> sprojsnd\<cdot> (srcdups\<cdot> (\<up>(ta,\<not> ack) \<bullet> tsAbs\<cdot> (tsSnd\<cdot>asa\<cdot>asc\<cdot> 
-   (Discr  ack))))) = \<up>ack \<bullet> sprojsnd\<cdot> (srcdups\<cdot> (\<up>(ta, \<not>ack) \<bullet> tsAbs\<cdot> (tsSnd\<cdot>asa\<cdot>asc\<cdot> (Discr  ack))))"
-        by auto
-      then have"srcdups\<cdot> (\<up>(\<not> ack) \<bullet> sprojsnd\<cdot> (srcdups\<cdot> (\<up>(ta, ack) \<bullet> tsAbs\<cdot> (tsSnd\<cdot>asa\<cdot>asc\<cdot> 
-                               (Discr (\<not> ack)))))) =  \<up>(\<not> ack) \<bullet> sprojsnd\<cdot> (srcdups\<cdot> (\<up>(ta, ack) \<bullet> 
-                                tsAbs\<cdot> (tsSnd\<cdot>asa\<cdot>asc\<cdot> (Discr (\<not> ack)))))"
-        by (insert f0 [of "\<not>ack"], auto)
-      then show "\<up>ack \<bullet> srcdups\<cdot> (\<up>(\<not> ack) \<bullet> sprojsnd\<cdot> (srcdups\<cdot> (\<up>(ta, ack) \<bullet> tsAbs\<cdot> (tsSnd\<cdot>asa\<cdot>asc\<cdot> 
-           (Discr (\<not> ack)))))) = \<up>ack \<bullet> \<up>(\<not> ack) \<bullet> sprojsnd\<cdot> (srcdups\<cdot> (\<up>(ta, ack) \<bullet> 
-                           tsAbs\<cdot> (tsSnd\<cdot>asa\<cdot>asc\<cdot> (Discr (\<not> ack)))))"
-      by simp
-    qed
-  qed 
-    
-lemma tssnd_alt_bit_h3:"i \<noteq> \<bottom> \<Longrightarrow> srcdups\<cdot>
-    (\<up>ack \<bullet> sprojsnd\<cdot>
-            (srcdups\<cdot>
-             (\<up>(ta, \<not> ack) \<bullet> tsAbs\<cdot>(tsSnd\<cdot>(tsMLscons\<cdot>(updis ta)\<cdot>i)\<cdot>as\<cdot>(Discr (\<not> ack)))))) =
-    \<up>ack \<bullet> sprojsnd\<cdot>
-           (srcdups\<cdot>(\<up>(ta, \<not> ack) \<bullet> tsAbs\<cdot>(tsSnd\<cdot>(tsMLscons\<cdot>(updis ta)\<cdot>i)\<cdot>as\<cdot>(Discr (\<not> ack)))))"
-  apply(induction as arbitrary: ack ta i,simp_all)
-  apply(subst srcdups_def [THEN fix_eq2], simp)
-  apply(simp add: tssnd_delayfun_nack_abs lscons_conv)
-  apply(case_tac "t=ack")
-  apply(simp add: tssnd_mlscons_nack_abs lscons_conv)
-  by(simp add: tssnd_mlscons_ack_abs lscons_conv tssnd_alt_bit_h4)
-
-lemma tssnd_alt_bit_h2:"
-       srcdups\<cdot>(sprojsnd\<cdot>(srcdups\<cdot>(\<up> (t, ack) \<bullet> tsAbs\<cdot>(tsSnd\<cdot>i\<cdot>as\<cdot>(Discr (\<not>ack)))))) =
-       sprojsnd\<cdot>(srcdups\<cdot>(\<up> (t, ack) \<bullet> tsAbs\<cdot>(tsSnd\<cdot>i\<cdot>as\<cdot>(Discr (\<not>ack)))))"
-  proof(induction i arbitrary: as ack t )
-  fix i:: "'a tstream" and as:: "bool tstream" and ack:: "bool discr" and t::"'a"
-    case adm
-    then show ?case
-    by simp
-  next
-    case bottom
-    then show ?case
-    by(simp add:lscons_conv)
-  next
-    case (delayfun asa)
-    then show ?case
-    apply(rule_tac ts=as in tscases, simp_all) 
-    apply(simp add: tssnd_delayfun_abs)
-    apply(case_tac "as=\<bottom>", simp_all)
-    by(simp add: tssnd_delayfun_msg_abs)
-  next
-    case (mlscons asa ta)
-    then show ?case
-    apply(rule_tac ts=as in tscases, simp_all) 
-    apply(simp add: tssnd_delayfun_nack_abs lscons_conv)
-    using tssnd_alt_bit_h3 apply blast
-    apply(case_tac "as=\<bottom>",simp_all)
-    apply(case_tac "a=(\<not> ack)")
-    apply(simp add: tssnd_mlscons_ack_abs lscons_conv)
-    using tssnd_alt_bit_h4 apply blast
-    apply(simp add: tssnd_mlscons_ack_abs lscons_conv)
-    by (simp add: lscons_conv tssnd_alt_bit_h3 tssnd_mlscons_nack_abs)  
-  qed
-
-lemma tssnd_alt_bit_h1:"i\<noteq>\<bottom> \<Longrightarrow> srcdups\<cdot>(sprojsnd\<cdot>(srcdups\<cdot>(\<up> (t, ack) \<bullet> tsAbs\<cdot>(tsSnd\<cdot>
-      (tsMLscons\<cdot>(updis t)\<cdot>i)\<cdot>as\<cdot>(Discr ack))))) = sprojsnd\<cdot>(srcdups\<cdot>(\<up> (t, ack) \<bullet> tsAbs\<cdot>(tsSnd\<cdot>
-      (tsMLscons\<cdot>(updis t)\<cdot>i)\<cdot>as\<cdot>(Discr ack))))"
-  apply(induction as arbitrary: i ack t, simp_all)
-  apply(simp add: tssnd_delayfun_nack_abs lscons_conv)
-  apply(rename_tac  ta i ack t )  
-  apply(case_tac "ta\<noteq>ack")
-  apply(simp add: tssnd_mlscons_nack_abs lscons_conv)
-  by(simp add: tssnd_mlscons_ack_abs lscons_conv tssnd_alt_bit_h2)
-
 lemma tssnd_alt_bit:
-  "tsAbs\<cdot>(tsRemDups\<cdot>(tsProjSnd\<cdot>(tsRemDups\<cdot>(tsSnd\<cdot>i\<cdot>as\<cdot>(Discr ack)))))
-    = tsAbs\<cdot>(tsProjSnd\<cdot>(tsRemDups\<cdot>(tsSnd\<cdot>i\<cdot>as\<cdot>(Discr ack))))"
-  apply(simp add: tsremdups_tsabs tsprojsnd_tsabs)
-  proof(induction i arbitrary: as ack, simp_all)
-  fix i:: "'a tstream" and as:: "bool tstream" and ack:: "bool discr"
-  case (delayfun i)
-  then show ?case
-    apply(rule_tac ts=as in tscases,simp_all)
-    apply(simp add: tssnd_delayfun_abs)
-    apply(case_tac "as=\<bottom>",simp_all)
-    by(simp add: tssnd_delayfun_msg_abs)  
-  next
-    case (mlscons i t)
-    then show ?case
-    apply(rule_tac ts=as in tscases,simp_all)
-    apply(simp add:tssnd_delayfun_nack_abs lscons_conv tssnd_alt_bit_h1)
-    apply(case_tac "as=\<bottom>",simp_all)
-    apply(case_tac "a=ack")
-    apply(simp add: tssnd_mlscons_ack_abs lscons_conv tssnd_alt_bit_h2)
-    by(simp add: tssnd_mlscons_nack_abs lscons_conv tssnd_alt_bit_h1)
-  qed
+  "tsAbs\<cdot>(tsRemDups\<cdot>(tsProjSnd\<cdot>(tsRemDups\<cdot>(tsSnd_h\<cdot>i\<cdot>as\<cdot>(Discr ack)))))
+    = tsAbs\<cdot>(tsProjSnd\<cdot>(tsRemDups\<cdot>(tsSnd_h\<cdot>i\<cdot>as\<cdot>(Discr ack))))"
+  oops
 
 text {* #fds = min{#i, #fas+1} where fds = map(\<alpha>.ds, \<Pi>1), fas = \<alpha>.as 
         when an acknowledgment is received then the next data next data element will eventually
         be transmitted given that there are more data elements to transmit *}
 lemma tssnd_ack2trans:
-  "#(tsAbs\<cdot>(tsProjFst\<cdot>(tsRemDups\<cdot>(tsSnd\<cdot>i\<cdot>as\<cdot>ack))))
+  "#\<surd>as = \<infinity> \<Longrightarrow> #(tsAbs\<cdot>(tsProjFst\<cdot>(tsRemDups\<cdot>(tsSnd_h\<cdot>i\<cdot>as\<cdot>ack))))
      = min (#(tsAbs\<cdot>i)) (lnsuc\<cdot>(#(tsAbs\<cdot>(tsRemDups\<cdot>as))))"
-oops
-
+  oops
 
 text {* #i > #fas \<Longrightarrow> #ds = \<infinity> where fas = \<alpha>.as
         if a data element is never acknowledged despite repetitive transmission by the sender 
         then the sender never stops transmitting this data element *}
 lemma tssnd_nack2inftrans:
-  "#(tsAbs\<cdot>i) > #(tsAbs\<cdot>(tsRemDups\<cdot>as)) \<Longrightarrow> #(tsAbs\<cdot>(tsSnd\<cdot>i\<cdot>as\<cdot>ack)) = \<infinity>"
-oops
+  "#\<surd>as = \<infinity> \<Longrightarrow> #(tsAbs\<cdot>i) > #(tsAbs\<cdot>(tsRemDups\<cdot>as)) \<Longrightarrow> #(tsAbs\<cdot>(tsSnd_h\<cdot>i\<cdot>as\<cdot>ack)) = \<infinity>"
+  oops
     
 end
